Adjust CTX

src/FrameStack/CTX.v
@@ -74,7 +74,7 @@ Definition CompatibleApp (R : nat -> Exp -> Exp -> Prop) :=
     list_biforall (R Γ) el el' ->
     R Γ (EApp e el) (EApp e' el').
 
-Definition CompatibleCase (R : nat -> Exp -> Exp -> Prop) := (* TODO: l or l' in places? *)
+Definition CompatibleCase (R : nat -> Exp -> Exp -> Prop) :=
   forall Γ e e' l l',
     EXP Γ ⊢ e ->
     EXP Γ ⊢ e' ->
@@ -134,6 +134,17 @@ Definition CompatibleTry (R : nat -> Exp -> Exp -> Prop) :=
     R (vl2 + Γ) e3 e3' ->
     R Γ (ETry e1 vl1 e2 vl2 e3) (ETry e1' vl1' e2' vl2' e3').
 
+Definition CompatibleReceive (R : nat -> Exp -> Exp -> Prop) :=
+  forall Γ l l',
+  Forall (fun '(p, g, e) => EXP PatListScope p + Γ ⊢ g /\ EXP PatListScope p + Γ ⊢ e) l ->
+  Forall (fun '(p, g, e) => EXP PatListScope p + Γ ⊢ g /\ EXP PatListScope p + Γ ⊢ e) l' ->
+  list_biforall (
+    fun '(p, g, e) '(p', g', e') =>
+      p = p' /\ R (PatListScope p + Γ) g g' /\
+      R (PatListScope p + Γ) e e'
+  ) l l' ->
+  R Γ (EReceive l) (EReceive l').
+
 Definition IsPreCtxRel (R : nat -> Exp -> Exp -> Prop) :=
   (forall Γ p1 p2, R Γ p1 p2 -> EXP Γ ⊢ p1 /\ EXP Γ ⊢ p2) /\
   Adequate R /\ IsReflexive R /\
@@ -150,7 +161,8 @@ Definition IsPreCtxRel (R : nat -> Exp -> Exp -> Prop) :=
   CompatibleLet R /\
   CompatibleSeq R /\
   CompatibleLetRec R /\
-  CompatibleTry R.
+  CompatibleTry R /\
+  CompatibleReceive R.
 
 Definition IsCtxRel (R : nat -> Exp -> Exp -> Prop) :=
   IsPreCtxRel R /\
@@ -248,6 +260,13 @@ Proof.
   * unfold CompatibleTry.
     intros.
     auto.
+  * unfold CompatibleReceive.
+    intros.
+    apply Erel_Receive_compat.
+    all: do 2 constructor; rewrite indexed_to_forall with (def := ([], `VNil,`VNil)) in H; rewrite indexed_to_forall with (def := ([], `VNil,`VNil)) in H0; intros.
+    all: rewrite map_nth with (d := ([], `VNil,`VNil)).
+    all: setoid_rewrite (map_nth (fst ∘ fst)) with (d := ([], `VNil,`VNil)).
+    all: (apply H0 in H2 + apply H in H2); destruct nth, p; simpl; try apply H2.
 Qed.
 
 Corollary CIU_IsPreCtxRel : IsPreCtxRel CIU_open.
@@ -324,6 +343,13 @@ Proof.
     apply CIU_iff_Rrel. apply Rrel_exp_compat.
     apply CIU_iff_Rrel, Rrel_exp_compat_reverse in H7, H8, H9.
     now apply Erel_IsPreCtxRel.
+  * intros ?; intros.
+    apply CIU_iff_Rrel. apply Rrel_exp_compat.
+    apply biforall_impl with (Q := fun '(p, g, e) '(p', g', e') =>
+        p = p' /\ Erel_open (PatListScope p + Γ) g g' /\ Erel_open (PatListScope p + Γ) e e') in H1. 2: { intros. destruct x, p, y, p, H2, H3.
+    apply CIU_iff_Rrel, Rrel_exp_compat_reverse in H3, H4.
+    intuition. }
+    now apply Erel_IsPreCtxRel.
 Qed.
 
 Inductive CtxIdent :=
@@ -336,25 +362,31 @@ Inductive CtxIdent :=
 
 Inductive Ctx :=
 | CHole
-| CFun     (vl : nat) (c : Ctx)
-| CParams  (ident : CtxIdent) (el : list Exp) (c : Ctx) (el' : list Exp)
-| CCons1   (c : Ctx) (tl : Exp)
-| CCons2   (hd : Exp) (c : Ctx)
-| CCallMod (c : Ctx) (f : Exp) (l : list Exp)
-| CCallFun (m : Exp) (c : Ctx) (l : list Exp)
-| CApp1    (c : Ctx) (l : list Exp)
-| CCase1   (c : Ctx) (l : list ((list Pat) * Exp * Exp))
-| CCase2   (e : Exp) (l : list ((list Pat) * Exp * Exp)) (lp : (list Pat)) (c : Ctx) (e2 : Exp) (l' : list ((list Pat) * Exp * Exp))
-| CCase3   (e : Exp) (l : list ((list Pat) * Exp * Exp)) (lp : (list Pat)) (e1 : Exp) (c : Ctx) (l' : list ((list Pat) * Exp * Exp))
-| CLet1    (l : nat) (c : Ctx) (e2 : Exp)
-| CLet2    (l : nat) (e1: Exp) (c : Ctx)
-| CSeq1    (c : Ctx) (e2 : Exp)
-| CSeq2    (e1 : Exp) (c : Ctx)
-| CLetRec1 (l : list (nat * Exp)) (n : nat) (c : Ctx) (l' : list (nat * Exp)) (e : Exp)
-| CLetRec2 (l : list (nat * Exp)) (c : Ctx)
-| CTry1    (c : Ctx) (vl1 : nat) (e2 : Exp) (vl2 : nat) (e3 : Exp)
-| CTry2    (e1 : Exp) (vl1 : nat) (c : Ctx) (vl2 : nat) (e3 : Exp)
-| CTry3    (e1 : Exp) (vl1 : nat) (e2 : Exp) (vl2 : nat) (c : Ctx)
+| CFun      (vl : nat) (c : Ctx)
+| CParams   (ident : CtxIdent) (el : list Exp) (c : Ctx) (el' : list Exp)
+| CCons1    (c : Ctx) (tl : Exp)
+| CCons2    (hd : Exp) (c : Ctx)
+| CCallMod  (c : Ctx) (f : Exp) (l : list Exp)
+| CCallFun  (m : Exp) (c : Ctx) (l : list Exp)
+| CApp1     (c : Ctx) (l : list Exp)
+| CCase1    (c : Ctx) (l : list ((list Pat) * Exp * Exp))
+| CCase2    (e : Exp) (l : list ((list Pat) * Exp * Exp))
+            (lp : (list Pat)) (c : Ctx) (e2 : Exp)  (l' : list ((list Pat) * Exp * Exp))
+| CCase3    (e : Exp) (l : list ((list Pat) * Exp * Exp))
+            (lp : (list Pat)) (e1 : Exp) (c : Ctx) (l' : list ((list Pat) * Exp * Exp))
+| CLet1     (l : nat) (c : Ctx) (e2 : Exp)
+| CLet2     (l : nat) (e1: Exp) (c : Ctx)
+| CSeq1     (c : Ctx) (e2 : Exp)
+| CSeq2     (e1 : Exp) (c : Ctx)
+| CLetRec1  (l : list (nat * Exp)) (n : nat) (c : Ctx) (l' : list (nat * Exp)) (e : Exp)
+| CLetRec2  (l : list (nat * Exp)) (c : Ctx)
+| CTry1     (c : Ctx) (vl1 : nat) (e2 : Exp) (vl2 : nat) (e3 : Exp)
+| CTry2     (e1 : Exp) (vl1 : nat) (c : Ctx) (vl2 : nat) (e3 : Exp)
+| CTry3     (e1 : Exp) (vl1 : nat) (e2 : Exp) (vl2 : nat) (c : Ctx)
+| CReceive1 (l : list ((list Pat) * Exp * Exp))
+            (lp : (list Pat)) (c : Ctx) (e2 : Exp) (l' : list ((list Pat) * Exp * Exp))
+| CReceive2 (l : list ((list Pat) * Exp * Exp))
+            (lp : (list Pat)) (e1 : Exp) (c : Ctx) (l' : list ((list Pat) * Exp * Exp))
 .
 
 Definition create_exp (ident : CtxIdent) (l : list Exp) :=
@@ -391,6 +423,8 @@ match C with
 | CTry1   c vl1 e2 vl2 e3  => EExp ( ETry (plug c p) vl1 e2 vl2 e3 )
 | CTry2   e1 vl1 c vl2 e3  => EExp ( ETry e1 vl1 (plug c p) vl2 e3 )
 | CTry3   e1 vl1 e2 vl2 c  => EExp ( ETry e1 vl1 e2 vl2 (plug c p) )
+| CReceive1 l lp c e2 l' => EExp ( EReceive (l ++ [(lp, (plug c p), e2)] ++ l') )
+| CReceive2 l lp e1 c l' => EExp ( EReceive (l ++ [(lp, e1, (plug c p))] ++ l') )
 end.
 
 Fixpoint plugc (C : Ctx) (p : Ctx) :=
@@ -415,6 +449,8 @@ match C with
 | CTry1   c vl1 e2 vl2 e3  => CTry1 (plugc c p) vl1 e2 vl2 e3
 | CTry2   e1 vl1 c vl2 e3  => CTry2 e1 vl1 (plugc c p) vl2 e3
 | CTry3   e1 vl1 e2 vl2 c  => CTry3 e1 vl1 e2 vl2 (plugc c p)
+| CReceive1 l lp c e2 l' => CReceive1 l lp (plugc c p) e2 l'
+| CReceive2 l lp e1 c l' => CReceive2 l lp e1 (plugc c p) l'
 end.
 
 
@@ -566,6 +602,20 @@ Inductive EECtxScope (Γh : nat) : nat -> Ctx -> Prop :=
   EECTX Γh ⊢ c ∷ (vl2 + Γ) ->
   EECTX Γh ⊢ (CTry3 e1 vl1 e2 vl2 c) ∷ Γ
 
+| CEScope_CReceive1 : forall Γ l lp c e2 l',
+  EXP PatListScope lp + Γ ⊢ e2 ->
+  Forall (fun '(p, g, e) => EXP PatListScope p + Γ ⊢ g /\ EXP PatListScope p + Γ ⊢ e) l ->
+  Forall (fun '(p, g, e) => EXP PatListScope p + Γ ⊢ g /\ EXP PatListScope p + Γ ⊢ e) l' ->
+  EECTX Γh ⊢ c ∷ ((PatListScope lp) + Γ) ->
+  EECTX Γh ⊢ (CReceive1 l lp c e2 l') ∷ Γ
+
+| CEScope_CReceive2 : forall Γ l lp e1 c l',
+  EXP (PatListScope lp + Γ) ⊢ e1 ->
+  Forall (fun '(p, g, e) => EXP PatListScope p + Γ ⊢ g /\ EXP PatListScope p + Γ ⊢ e) l ->
+  Forall (fun '(p, g, e) => EXP PatListScope p + Γ ⊢ g /\ EXP PatListScope p + Γ ⊢ e) l' ->
+  EECTX Γh ⊢ c ∷ ((PatListScope lp) + Γ) ->
+  EECTX Γh ⊢ (CReceive2 l lp e1 c l') ∷ Γ
+
 where
 "'EECTX' Γh ⊢ C ∷ Γ" := (EECtxScope Γh Γ C)
 .
@@ -641,6 +691,34 @@ Proof.
   * do 2 constructor. 2: now apply IHC.
     intros. rewrite indexed_to_forall with (def := (0, `VNil)) in H4. apply H4 in H.
     do 2 rewrite map_nth with (d := (0, `VNil)). now destruct nth.
+  * do 2 constructor; auto; rewrite indexed_to_forall with (def := ([], `VNil, `VNil)) in H8, H9.
+    all: intros; rewrite map_nth with (d := ([], `VNil, `VNil));
+    extract_map_fun F; replace [] with (F ([], `VNil, `VNil)) at 1 by now subst F.
+    rewrite map_nth. 2: rewrite map_nth.
+    all: subst F.
+    all: apply nth_possibilities_alt with (def := ([], `VNil, `VNil)) in H; intuition.
+    - apply H8 in H2. destruct nth, p, nth, p. inv H. cbn. apply H2.
+    - simpl in H1. rewrite app_nth2; auto. remember (i - length l) as i'.
+      destruct i'; cbn. now apply IHC.
+      specialize (H9 i' ltac:(lia)). destruct nth, p. apply H9.
+    - rewrite app_nth1; auto. specialize (H8 i ltac:(lia)). destruct nth, p. apply H8.
+    - simpl in H1. rewrite app_nth2; auto. remember (i - length l) as i'.
+      destruct i'; cbn. auto.
+      specialize (H9 i' ltac:(lia)). destruct nth, p. apply H9.
+  * do 2 constructor; auto; rewrite indexed_to_forall with (def := ([], `VNil, `VNil)) in H8, H9.
+    all: intros; rewrite map_nth with (d := ([], `VNil, `VNil));
+    extract_map_fun F; replace [] with (F ([], `VNil, `VNil)) at 1 by now subst F.
+    rewrite map_nth. 2: rewrite map_nth.
+    all: subst F.
+    all: apply nth_possibilities_alt with (def := ([], `VNil, `VNil)) in H; intuition.
+    - apply H8 in H2. destruct nth, p, nth, p. inv H. cbn. apply H2.
+    - simpl in H1. rewrite app_nth2; auto. remember (i - length l) as i'.
+      destruct i'; cbn. auto.
+      specialize (H9 i' ltac:(lia)). destruct nth, p. apply H9.
+    - rewrite app_nth1; auto. specialize (H8 i ltac:(lia)). destruct nth, p. apply H8.
+    - simpl in H1. rewrite app_nth2; auto. remember (i - length l) as i'.
+      destruct i'; cbn. now apply IHC.
+      specialize (H9 i' ltac:(lia)). destruct nth, p. apply H9.
 Qed.
 
 Lemma plugc_preserves_scope_exp : forall {Γh Couter Γ Cinner Γ'},
@@ -688,7 +766,7 @@ Lemma CTX_bigger : forall R' : nat -> Exp -> Exp -> Prop,
     IsPreCtxRel R' -> forall (Γ : nat) (e1 e2 : Exp), R' Γ e1 e2 -> CTX Γ e1 e2.
 Proof.
   intros R' HR.
-  destruct HR as [Rscope [Radequate [Rrefl [Rtrans [RFun [ RValues [RCons [RTuple [RMap  [ RCall [ RPrimOp [RApp [RCase [RLet [RSeq [RLetRec RTry ] ] ] ] ] ] ] ] ] ] ] ] ] ] ] ].
+  destruct HR as [Rscope [Radequate [Rrefl [Rtrans [RFun [ RValues [RCons [RTuple [RMap  [ RCall [ RPrimOp [RApp [RCase [RLet [RSeq [RLetRec [RTry RReceive] ] ] ] ] ] ] ] ] ] ] ] ] ] ] ] ].
   unfold CTX.
   intros.
   destruct (Rscope _ _ _ H) as [Hscope_e1 Hscope_e2].
@@ -810,6 +888,32 @@ Proof.
     - apply RTry; auto.
       + eapply @plug_preserves_scope_exp with (e := e1) in H9; eauto 2.
       + eapply @plug_preserves_scope_exp with (e := e2) in H9; eauto 2.
+    - apply RReceive; auto.
+      1-2: apply Forall_app; split; auto; constructor; auto.
+      1-2: simpl; split; try eapply plug_preserves_scope_exp; eauto.
+      apply biforall_app. 2: constructor.
+      + apply forall_biforall_refl, Forall_forall. intros.
+        rewrite Forall_forall in H8. destruct x, p. split. 2: split.
+        reflexivity.
+        all: apply Rrefl; now apply H8 in H0.
+      + split; auto.
+      + apply forall_biforall_refl, Forall_forall. intros.
+        rewrite Forall_forall in H9. destruct x, p. split. 2: split.
+        reflexivity.
+        all: apply Rrefl; now apply H9 in H0.
+    - apply RReceive; auto.
+      1-2: apply Forall_app; split; auto; constructor; auto.
+      1-2: simpl; split; try eapply plug_preserves_scope_exp; eauto.
+      apply biforall_app. 2: constructor.
+      + apply forall_biforall_refl, Forall_forall. intros.
+        rewrite Forall_forall in H8. destruct x, p. split. 2: split.
+        reflexivity.
+        all: apply Rrefl; now apply H8 in H0.
+      + split; auto.
+      + apply forall_biforall_refl, Forall_forall. intros.
+        rewrite Forall_forall in H9. destruct x, p. split. 2: split.
+        reflexivity.
+        all: apply Rrefl; now apply H9 in H0.
   }
   now apply H2.
 Qed.
@@ -987,6 +1091,72 @@ Proof.
     1: rewrite app_length; slia.
     all: auto.
     apply Forall_app; split; auto.
+Qed.
+
+Theorem CTX_isPreCtxRel_CReceive Γ tl tl' pl g g' b' b hds :
+  list_biforall
+        (fun '(p, g, e) '(p', g', e') =>
+         p = p' /\
+         ((EXP PatListScope p + Γ ⊢ g /\ EXP PatListScope p + Γ ⊢ g') /\
+          (forall C : Ctx,
+           EECTX PatListScope p + Γ ⊢ C ∷ 0 ->
+           | [], plug C g | ↓ -> | [], plug C g' | ↓)) /\
+         (EXP PatListScope p + Γ ⊢ e /\ EXP PatListScope p + Γ ⊢ e') /\
+         (forall C : Ctx,
+          EECTX PatListScope p + Γ ⊢ C ∷ 0 ->
+          | [], plug C e | ↓ -> | [], plug C e' | ↓)) tl tl' ->
+   EXP PatListScope pl + Γ ⊢ g ->
+   EXP PatListScope pl + Γ ⊢ b ->
+   EXP PatListScope pl + Γ ⊢ g' ->
+   EXP PatListScope pl + Γ ⊢ b' ->
+   (forall C : Ctx,
+      EECTX PatListScope pl + Γ ⊢ C ∷ 0 ->
+      | [], plug C b | ↓ -> | [], plug C b' | ↓) ->
+   (forall C : Ctx,
+      EECTX PatListScope pl + Γ ⊢ C ∷ 0 ->
+      | [], plug C g | ↓ -> | [], plug C g' | ↓) ->
+  Forall (fun '(p, g, e) => EXP PatListScope p + Γ ⊢ g /\ EXP PatListScope p + Γ ⊢ e) hds ->
+  forall C, EECTX Γ ⊢ C ∷ 0 ->
+  | [], plug (plugc C (CReceive1 hds pl CHole b tl)) g | ↓ ->
+  | [], plug C (° EReceive (hds ++ (pl, g', b') :: tl')) | ↓.
+Proof.
+  intros IH. revert hds g b g' b' pl. induction IH; intros.
+  * apply H4 in H7.
+    2: {
+      eapply plugc_preserves_scope_exp; eauto.
+      constructor; auto. constructor.
+    }
+    replace (plug (plugc C (CReceive1 hds pl CHole b [])) g') with
+            (plug (plugc C (CReceive2 hds pl g' CHole [])) b) in H7
+      by now repeat rewrite <- plug_assoc.
+    apply H3 in H7. now rewrite <- plug_assoc in H7.
+    eapply plugc_preserves_scope_exp; eauto.
+    constructor; auto. constructor.
+  * destruct hd as [p2 b2], p2 as [pl2 g2], hd' as [p2' b2'], p2' as [pl2' g2']. intuition.
+    subst.
+    apply H5 in H8.
+    2: {
+      eapply plugc_preserves_scope_exp; eauto.
+      constructor; auto; constructor; intuition.
+      clear -IH. induction IH; constructor; destruct hd, p, hd', p; intuition.
+    }
+    replace (plug (plugc C (CReceive1 hds pl CHole b ((pl2', g2, b2) :: tl))) g') with
+            (plug (plugc C (CReceive2 hds pl g' CHole ((pl2', g2, b2) :: tl))) b) in H8
+      by now repeat rewrite <- plug_assoc.
+    apply H4 in H8.
+    2: {
+      eapply plugc_preserves_scope_exp; eauto.
+      constructor; auto; constructor; intuition.
+      clear -IH. induction IH; constructor; destruct hd, p, hd', p; intuition.
+    }
+    replace (plug (plugc C (CReceive2 hds pl g' CHole ((pl2', g2, b2) :: tl))) b') with
+            (plug (plugc C (CReceive1 (hds ++ [(pl, g', b')]) pl2' CHole b2 tl)) g2) in H8.
+    2: { repeat rewrite <- plug_assoc. cbn. now rewrite <- app_assoc. }
+    replace (hds ++ (pl, g', b') :: (pl2', g2', b2') :: tl') with
+            ((hds ++ [(pl, g', b')]) ++ (pl2', g2', b2') :: tl')
+      by now rewrite <- app_assoc.
+    eapply IHIH. 5: exact H13. 5: exact H12. all: eauto.
+    apply Forall_app; intuition.
 Qed.
 
 Lemma CTX_IsPreCtxRel : IsPreCtxRel CTX.
@@ -1284,6 +1454,27 @@ Proof.
     apply H13 in H17.
     rewrite <- plug_assoc in H17. simpl in H17. now subst.
     eapply plugc_preserves_scope_exp; eauto; constructor; auto; constructor.
+  * unfold CompatibleReceive. intros. subst. unfold CTX in *. intuition.
+    (* scopes: *)
+    1-2: do 2 constructor; auto; rewrite indexed_to_forall with (def := ([], `VNil, `VNil)) in H, H0; intros i Hlen;
+         try setoid_rewrite map_nth with (d := ([], `VNil, `VNil));
+         try setoid_rewrite (map_nth (fst ∘ fst)) with (d := ([], `VNil, `VNil));
+         try setoid_rewrite (map_nth (snd ∘ fst)) with (d := ([], `VNil, `VNil));
+         apply biforall_length in H1;
+         try apply H in Hlen as Hlen1; try apply H0 in Hlen as Hlen2;
+         rewrite <- H1 in H0;
+         try apply H in Hlen as Hlen1; try apply H0 in Hlen as Hlen2;
+         destruct nth, p; now cbn in *.
+    (* plug assoc *)
+    inv H1.
+    - assumption.
+    - destruct hd as [p b], p as [pl g], hd' as [p' b'], p' as [pl' g'].
+      intuition. subst.
+      replace (plug C (° EReceive ((pl', g, b) :: tl))) with
+              (plug (plugc C (CReceive1 [] pl' CHole b tl)) g) in H3
+        by now repeat rewrite <- plug_assoc.
+      eapply CTX_isPreCtxRel_CReceive with (hds := []).
+      eassumption. 5-6: eassumption. all: auto.
 Qed.
 
 Lemma CTX_IsCtxRel : IsCtxRel CTX.
@@ -1506,10 +1697,17 @@ Proof.
            constructor. split; auto. split; simpl; auto.
            now apply CTX_refl. constructor; auto.
            split; auto. split; simpl; apply CTX_refl; auto.
-           1: scope_solver.
-           do 2 constructor.
+           1: {
+             (* NOTE: scope_solver does not terminate here *)
+             do 2 constructor; auto.
+             2-3: intros; rewrite Nat.add_0_r.
+             2-3: now (apply H17 + apply H18).
+             do 2 constructor. apply indexed_to_forall.
+             now apply Valscope_lift.
+           }
+           (* do 2 constructor.
            1: do 2 constructor; now apply indexed_to_forall, Valscope_lift.
-           1-2: intros; rewrite Nat.add_0_r; try apply H20; now try apply H21.
+           1-2: intros; rewrite Nat.add_0_r; try apply H20; now try apply H21. *)
         -- simpl. apply CTX_IsPreCtxRel; auto.
            all: rewrite Nat.add_0_r; auto. all: now apply CTX_refl.
         -- simpl. apply CTX_IsPreCtxRel; auto. now apply CTX_refl.
